reorganize

Core/Node.v
@@ -3,11 +3,347 @@ Require Import ssreflect ssrbool ssrnat eqtype ssrfun seq fintype div path.
 Require Import Eqdep Relations.
 From fcsl
 Require Import pred prelude ordtype pcm finmap unionmap heap.
-From CasperToychain
-Require Import Blockforest.
 Set Implicit Arguments.
 Unset Strict Implicit.
 Unset Printing Implicit Defensive.
+
+Parameter byte : ordType.
+Parameter Address : finType.
+
+Inductive Sender :=
+| NullSender : Sender
+| AddrSender : Address -> Sender.
+
+Definition eq_Sender (s s' : Sender) :=
+  match s, s' with
+  | NullSender, NullSender => true
+  | NullSender, _ => false
+  | AddrSender a1, AddrSender a2 => a1 == a2
+  | AddrSender _, _ => false
+  end.
+
+Lemma eq_SenderP : Equality.axiom eq_Sender.
+Proof.
+case => [|a1]; case => [|a2].
+- by constructor 1.
+- by constructor 2.
+- by constructor 2.
+- rewrite /eq_Sender /=.
+  case H1: (a1 == a2); [move/eqP: H1=>?; subst a2| constructor 2];
+    last by case=>?; subst a2;rewrite eqxx in H1.
+  by constructor 1.
+Qed.
+
+Definition Sender_eqMixin :=
+  Eval hnf in EqMixin eq_SenderP.
+Canonical Sender_eqType :=
+  Eval hnf in EqType Sender Sender_eqMixin.
+
+Record AttestationRecord {Hash : ordType} :=
+  mkAR {
+    slot_ar : nat;
+    shard_id : nat;
+    oblique_parent_hashes : seq Hash;
+    shard_block_hash : Hash;
+    attester_bitfield : seq byte;
+    aggregate_sig : seq nat
+  }.
+
+Record Block {Hash : ordType} :=
+  mkB {
+    (* Hash of the parent block *)
+    parent_hash : Hash;
+    (* Slot number (for the PoS mechanism) *)
+    slot_number : nat;
+    (* Randao commitment reveal *)
+    randao_reveal : Hash;
+    (* Attestations *)
+    attestations : seq (@AttestationRecord Hash);
+    (* Reference to PoW chain block *)
+    pow_chain_ref : Hash;
+    (* Hash of the active state *)
+    active_state_root : Hash;
+    (* Hash of the crystallized state *)
+    crystallized_state_root : Hash;
+  }.
+
+Record ShardAndCommittee :=
+  mkSAC {
+    (* The shard ID *)
+    shard_id_sac : nat;
+    (* Validator indices *)
+    committee : seq nat
+  }.
+
+Record CrosslinkRecord {Hash : ordType} :=
+  mkCR {
+    (* What dynasty the crosslink was submitted in *)
+    dynasty : nat;
+    (* slot during which crosslink was added *)
+    slot : nat;
+    (* The block hash *)
+    hash : Hash
+  }.
+
+Record ValidatorRecord {Hash : ordType} :=
+  mkVR {
+    (* The validator's public key *)
+    pubkey : nat;
+    (* What shard the validators balance will be sent to after withdrawal *)
+    withdrawal_shard : nat;
+    (* And what address *)
+    withdrawal_address : Sender;
+    (* The validators current RANDAO beacon commitment *)
+    randao_commitment : Hash;
+    (* Current balance *)
+    balance : nat;
+    (* Dynasty where the validator is inducted *)
+    start_dynasty : nat;
+    (* Dynasty where the validator leaves *)
+    end_dynasty : nat
+  }.
+
+Record ActiveState {Hash : ordType} :=
+  mkAS {
+    (* Attestations that have not yet been processed *)
+    pending_attestations : seq (@AttestationRecord Hash);
+    (* Most recent 2*CYCLE_LENGTH block hashes, older to newer *)
+    recent_block_hashes : seq Hash;
+    (* TODO: need to have block_vote_cache and chain here? *)
+  }.
+
+Record CrystallizedState {Hash : ordType} :=
+  mkCS {
+    (* List of validators *)
+    validators: seq (@ValidatorRecord Hash);
+    (* Last CrystallizedState recalculation *)
+    last_state_recalc: nat;
+    (* What active validators are part of the attester set *)
+    (* at what height; and in what shard. Starts at slot *)
+    (* last_state_recalc - CYCLE_LENGTH *)
+    shard_and_committee_for_slots: seq (seq ShardAndCommittee);
+    (* The last justified slot *)
+    last_justified_slot: nat;
+    (* Number of consecutive justified slots ending at this one *)
+    justified_streak: nat;
+    (* The last finalized slot *)
+    last_finalized_slot: nat;
+    (* The current dynasty *)
+    current_dynasty: nat;
+    (* Records about the most recent crosslink for each shard *)
+    crosslink_records: seq (@CrosslinkRecord Hash);
+    (* Used to select the committees for each shard *)
+    dynasty_seed: Hash;
+    (* Last epoch the crosslink seed was reset *)
+    dynasty_start: nat;
+  }.
+
+Definition eq_validator_record {H : ordType} (vr vr' : @ValidatorRecord H) :=
+  match vr, vr' with
+  | mkVR pk ws wa rc b sd ed, mkVR pk' ws' wa' rc' b' sd' ed' =>
+    [&& pk == pk', ws == ws', wa == wa', rc == rc', b == b', sd == sd' & ed == ed']
+  end.
+
+Lemma eq_validator_recordP {H : ordType} : Equality.axiom (@eq_validator_record H).
+case=> pk ws wa rc b sd ed; case=> pk' ws' wa' rc' b' sd' ed'; rewrite /eq_validator_record/=.
+case H2: (pk == pk'); [move/eqP: H2=>?; subst pk'| constructor 2];
+  last by case=>?; subst pk';rewrite eqxx in H2.
+case H3: (ws == ws'); [move/eqP: H3=>?; subst ws'| constructor 2];
+  last by case=>?; subst ws';rewrite eqxx in H3.
+case H4: (wa == wa'); [move/eqP: H4=>?; subst wa'| constructor 2];
+  last by case=>?; subst wa';rewrite eqxx in H4.
+case H5: (rc == rc'); [move/eqP: H5=>?; subst rc'| constructor 2];
+  last by case=>?; subst rc';rewrite eqxx in H5.
+case H6: (b == b'); [move/eqP: H6=>?; subst b'| constructor 2];
+  last by case=>?; subst b';rewrite eqxx in H6.
+case H7: (sd == sd'); [move/eqP: H7=>?; subst sd'| constructor 2];
+  last by case=>?; subst sd';rewrite eqxx in H7.
+case H8: (ed == ed'); [move/eqP: H8=>?; subst ed'| constructor 2];
+  last by case=>?; subst ed';rewrite eqxx in H8.
+by constructor 1.
+Qed.
+
+Canonical ValidatorRecord_eqMixin {H : ordType} :=
+  Eval hnf in EqMixin (@eq_validator_recordP H).
+Canonical ValidatorRecord_eqType {H : ordType} :=
+  Eval hnf in EqType (@ValidatorRecord H) (@ValidatorRecord_eqMixin H).
+
+Definition eq_attestation_record {H : ordType} (ar ar' : @AttestationRecord H) :=
+  match ar, ar' with
+  | mkAR sa si oph sbh ab ags, mkAR sa' si' oph' sbh' ab' ags' =>
+    [&& sa == sa', si == si', oph == oph', sbh == sbh', ab == ab' & ags == ags']
+  end.
+
+Lemma eq_attestation_recordP {H : ordType} : Equality.axiom (@eq_attestation_record H).
+Proof.
+case=> sa si oph sbh ab ags; case=> sa' si' oph' sbh' ab' ags'; rewrite /eq_attestation_record/=.
+case H2: (sa == sa'); [move/eqP: H2=>?; subst sa'| constructor 2];
+  last by case=>?; subst sa';rewrite eqxx in H2.
+case H3: (si == si'); [move/eqP: H3=>?; subst si'| constructor 2];
+  last by case=>?; subst si';rewrite eqxx in H3.
+case H4: (oph == oph'); [move/eqP: H4=>?; subst oph'| constructor 2];
+  last by case=>?; subst oph';rewrite eqxx in H4.
+case H5: (sbh == sbh'); [move/eqP: H5=>?; subst sbh'| constructor 2];
+  last by case=>?; subst sbh';rewrite eqxx in H5.
+case H6: (ab == ab'); [move/eqP: H6=>?; subst ab'| constructor 2];
+  last by case=>?; subst ab';rewrite eqxx in H6.
+case H7: (ags == ags'); [move/eqP: H7=>?; subst ags'| constructor 2];
+  last by case=>?; subst ags';rewrite eqxx in H7.
+by constructor 1.
+Qed.
+
+Canonical AttestationRecord_eqMixin {H : ordType} :=
+  Eval hnf in EqMixin (@eq_attestation_recordP H).
+Canonical AttestationRecord_eqType {H : ordType} :=
+  Eval hnf in EqType (@AttestationRecord H) (@AttestationRecord_eqMixin H).
+
+Definition eq_block {H : ordType} (b b' : @Block H) :=
+  match b, b' with
+  | mkB ph sn rr ars pcr asr csr, mkB ph' sn' rr' ars' pcr' asr' csr' =>
+    [&& ph == ph', sn == sn', rr == rr', ars == ars', pcr == pcr', asr == asr' & csr == csr']
+  end.
+      
+Lemma eq_blockP {H : ordType} : Equality.axiom (@eq_block H).
+Proof.
+case=> ph sn rr ars pcr asr csr;
+case=> ph' sn' rr' ars' pcr' asr' csr'; rewrite /eq_block/=.
+case H2: (ph == ph'); [move/eqP: H2=>?; subst ph'| constructor 2];
+  last by case=>?; subst ph';rewrite eqxx in H2.
+case H3: (sn == sn'); [move/eqP: H3=>?; subst sn'| constructor 2];
+  last by case=>?; subst sn';rewrite eqxx in H3.
+case H4: (rr == rr'); [move/eqP: H4=>?; subst rr'| constructor 2];
+  last by case=>?; subst rr';rewrite eqxx in H4.
+case H5: (ars == ars'); [move/eqP: H5=>?; subst ars'| constructor 2];
+  last by case=>?; subst ars';rewrite eqxx in H5.
+case H6: (pcr == pcr'); [move/eqP: H6=>?; subst pcr'| constructor 2];
+  last by case=>?; subst pcr';rewrite eqxx in H6.
+case H7: (asr == asr'); [move/eqP: H7=>?; subst asr'| constructor 2];
+  last by case=>?; subst asr';rewrite eqxx in H7.
+case H8: (csr == csr'); [move/eqP: H8=>?; subst csr'| constructor 2];
+  last by case=>?; subst csr';rewrite eqxx in H8.
+by constructor 1. 
+Qed.
+
+Canonical Block_eqMixin {H : ordType} :=
+  Eval hnf in EqMixin (@eq_blockP H ).
+Canonical Block_eqType {H : ordType} :=
+  Eval hnf in EqType (@Block H) (@Block_eqMixin H).
+
+Parameter Hash : finType.
+Parameter NodeId : finType.
+Parameter Timestamp : Type.
+
+Definition Hash_ordMixin := fin_ordMixin Hash.
+Canonical Hash_finType := Eval hnf in OrdType Hash Hash_ordMixin.
+
+Definition block := @Block [ordType of Hash].
+
+Parameter GenesisBlock : block.
+
+Definition Blockforest := union_map [ordType of Hash] block.
+
+Parameter hashB : block -> Hash.
+
+Axiom hashB_inj : injective hashB.
+
+Notation "# b" := (hashB b) (at level 20).
+
+Definition get_block (bf : Blockforest) k : Block :=
+  if find k bf is Some b then b else GenesisBlock.
+
+Definition has_init_block (bf : Blockforest) :=
+  find (# GenesisBlock) bf = Some GenesisBlock.
+
+Definition bfExtend (bf : Blockforest) (b : block) :=
+  if #b \in dom bf then bf else #b \\-> b \+ bf.
+
+Definition validH (bf : Blockforest) :=
+  forall h b, find h bf = Some b -> h = hashB b.
+
+Lemma bfExtendV bf b : valid bf = valid (bfExtend bf b).
+Proof.
+rewrite /bfExtend; case: ifP=>//N.
+by rewrite validPtUn/= N andbC.
+Qed.
+
+Lemma bfExtendH bf b : valid bf -> validH bf -> validH (bfExtend bf b).
+Proof.
+move=>V H z c; rewrite /bfExtend.
+case: ifP=>X; first by move/H.
+rewrite findUnL ?validPtUn ?V ?X//.
+case: ifP=>Y; last by move/H.
+rewrite domPt inE in Y; move/eqP: Y=>Y; subst z.
+by rewrite findPt; case=>->.
+Qed.
+
+Lemma bfExtendIB bf b :
+  valid bf -> validH bf -> has_init_block bf ->
+  has_init_block (bfExtend bf b).
+Proof.
+move=>V H; rewrite /bfExtend/has_init_block=>Ib.
+case: ifP=>X; first done.
+rewrite findUnL ?validPtUn ?V ?X//.
+case: ifP=>Y; last done.
+rewrite domPt inE in Y; move/eqP: Y=>Y.
+by specialize (hashB_inj Y)=><-; rewrite Y findPt.
+Qed.
+
+(* HELPERS *)
+
+Definition set_crystallized_state_validators a v := @mkCS [ordType of Hash] v (last_state_recalc a) (shard_and_committee_for_slots a) (last_justified_slot a) (justified_streak a) (last_finalized_slot a) (current_dynasty a) (crosslink_records a) (dynasty_seed a) (dynasty_start a).
+Definition set_crystallized_state_last_state_recalc a v := @mkCS [ordType of Hash] (validators a) v (shard_and_committee_for_slots a) (last_justified_slot a) (justified_streak a) (last_finalized_slot a) (current_dynasty a) (crosslink_records a) (dynasty_seed a) (dynasty_start a).
+Definition set_crystallized_state_shard_and_committee_for_slots a v := @mkCS [ordType of Hash] (validators a) (last_state_recalc a) v (last_justified_slot a) (justified_streak a) (last_finalized_slot a) (current_dynasty a) (crosslink_records a) (dynasty_seed a) (dynasty_start a).
+Definition set_crystallized_state_last_justified_slot a v := @mkCS [ordType of Hash] (validators a) (last_state_recalc a) (shard_and_committee_for_slots a) v (justified_streak a) (last_finalized_slot a) (current_dynasty a) (crosslink_records a) (dynasty_seed a) (dynasty_start a).
+Definition set_crystallized_state_justified_streak a v := @mkCS [ordType of Hash] (validators a) (last_state_recalc a) (shard_and_committee_for_slots a) (last_justified_slot a) v (last_finalized_slot a) (current_dynasty a) (crosslink_records a) (dynasty_seed a) (dynasty_start a).
+Definition set_crystallized_state_last_finalized_slot a v := @mkCS [ordType of Hash] (validators a) (last_state_recalc a) (shard_and_committee_for_slots a) (last_justified_slot a) (justified_streak a) v (current_dynasty a) (crosslink_records a) (dynasty_seed a) (dynasty_start a).
+Definition set_crystallized_state_current_dynasty a v := @mkCS [ordType of Hash] (validators a) (last_state_recalc a) (shard_and_committee_for_slots a) (last_justified_slot a) (justified_streak a) (last_finalized_slot a) v (crosslink_records a) (dynasty_seed a) (dynasty_start a).
+Definition set_crystallized_state_crosslink_records a v := @mkCS [ordType of Hash] (validators a) (last_state_recalc a) (shard_and_committee_for_slots a) (last_justified_slot a) (justified_streak a) (last_finalized_slot a) (current_dynasty a) v (dynasty_seed a) (dynasty_start a).
+Definition set_crystallized_state_dynasty_seed a v := @mkCS [ordType of Hash] (validators a) (last_state_recalc a) (shard_and_committee_for_slots a) (last_justified_slot a) (justified_streak a) (last_finalized_slot a) (current_dynasty a) (crosslink_records a) v (dynasty_start a).
+Definition set_crystallized_state_dynasty_start a v := @mkCS [ordType of Hash] (validators a) (last_state_recalc a) (shard_and_committee_for_slots a) (last_justified_slot a) (justified_streak a) (last_finalized_slot a) (current_dynasty a) (crosslink_records a) (dynasty_seed a) v.
+
+Notation "{[ a 'with' 'validators' := v ]}" := (set_crystallized_state_validators a v).
+Notation "{[ a 'with' 'last_state_recalc' := v ]}" := (set_crystallized_state_last_state_recalc a v).
+Notation "{[ a 'with' 'shard_and_committee_for_slots' := v ]}" := (set_crystallized_state_shard_and_committee_for_slots a v).
+Notation "{[ a 'with' 'last_justified_slot' := v ]}" := (set_crystallized_state_last_justified_slot a v).
+Notation "{[ a 'with' 'justified_streak' := v ]}" := (set_crystallized_state_justified_streak a v).
+Notation "{[ a 'with' 'last_finalized_slot' := v ]}" := (set_crystallized_state_last_finalized_slot a v).
+Notation "{[ a 'with' 'current_dynasty' := v ]}" := (set_crystallized_state_current_dynasty a v).
+Notation "{[ a 'with' 'crosslink_records' := v ]}" := (set_crystallized_state_crosslink_records a v).
+Notation "{[ a 'with' 'dynasty_seed' := v ]}" := (set_crystallized_state_dynasty_seed a v).
+Notation "{[ a 'with' 'dynasty_start' := v ]}" := (set_crystallized_state_dynasty_start a v).
+
+Arguments set_crystallized_state_validators  _ _/.
+Arguments set_crystallized_state_last_state_recalc  _ _/.
+Arguments set_crystallized_state_shard_and_committee_for_slots  _ _/.
+Arguments set_crystallized_state_last_justified_slot  _ _/.
+Arguments set_crystallized_state_justified_streak  _ _/.
+Arguments set_crystallized_state_last_finalized_slot  _ _/.
+Arguments set_crystallized_state_current_dynasty  _ _/.
+Arguments set_crystallized_state_crosslink_records  _ _/.
+Arguments set_crystallized_state_dynasty_seed  _ _/.
+Arguments set_crystallized_state_dynasty_start  _ _/.
+
+Definition set_validator_record_pubkey a v := @mkVR [ordType of Hash] v (withdrawal_shard a) (withdrawal_address a) (randao_commitment a) (balance a) (start_dynasty a) (end_dynasty a).
+Definition set_validator_record_withdrawal_shard a v := @mkVR [ordType of Hash] (pubkey a) v (withdrawal_address a) (randao_commitment a) (balance a) (start_dynasty a) (end_dynasty a).
+Definition set_validator_record_withdrawal_address a v := @mkVR [ordType of Hash] (pubkey a) (withdrawal_shard a) v (randao_commitment a) (balance a) (start_dynasty a) (end_dynasty a).
+Definition set_validator_record_randao_commitment a v := @mkVR [ordType of Hash] (pubkey a) (withdrawal_shard a) (withdrawal_address a) v (balance a) (start_dynasty a) (@end_dynasty [ordType of Hash] a).
+Definition set_validator_record_balance a v := @mkVR [ordType of Hash] (pubkey a) (withdrawal_shard a) (withdrawal_address a) (randao_commitment a) v (start_dynasty a) (end_dynasty a).
+Definition set_validator_record_start_dynasty a v := @mkVR [ordType of Hash] (pubkey a) (withdrawal_shard a) (withdrawal_address a) (randao_commitment a) (balance a) v (end_dynasty a).
+Definition set_validator_record_end_dynasty a v := @mkVR [ordType of Hash] (pubkey a) (withdrawal_shard a) (withdrawal_address a) (randao_commitment a) (balance a) (start_dynasty a) v.
+
+Notation "{[ a 'with' 'pubkey' := v ]}" := (set_validator_record_pubkey a v).
+Notation "{[ a 'with' 'withdrawal_shard' := v ]}" := (set_validator_record_withdrawal_shard a v).
+Notation "{[ a 'with' 'withdrawal_address' := v ]}" := (set_validator_record_withdrawal_address a v).
+Notation "{[ a 'with' 'balance' := v ]}" := (set_validator_record_balance a v).
+Notation "{[ a 'with' 'start_dynasty' := v ]}" := (set_validator_record_start_dynasty a v).
+Notation "{[ a 'with' 'end_dynasty' := v ]}" := (set_validator_record_end_dynasty a v).
+
+Arguments set_validator_record_pubkey  _ _/.
+Arguments set_validator_record_withdrawal_shard  _ _/.
+Arguments set_validator_record_withdrawal_address  _ _/.
+Arguments set_validator_record_balance  _ _/.
+Arguments set_validator_record_start_dynasty  _ _/.
+Arguments set_validator_record_end_dynasty  _ _/.
 
 Definition NodeId_ordMixin := fin_ordMixin NodeId.
 Canonical NodeId_ordType := Eval hnf in OrdType NodeId NodeId_ordMixin.
